MasterThesis/Compiler/Proofs/Commons.lean
@@ -5,22 +5,22 @@ import MasterThesis.SCORE.Proofs.Language
 import MasterThesis.LOOP.Proofs.Language
 import MasterThesis.Compiler.Commons
 
-lemma eq_states_update {σ : LOOP.Store} {τ : SCORE.Store} (x : Ident) (v : ℕ) : some σ =ₛ some τ → some ([x ↦ v] σ) =ₛ some ([x ↦ ↑v :: τ x] τ) := by
+lemma eq_states_update {σ : LOOP.Store} {τ : SCORE.Store} (x : Ident) (v : ℕ) : some σ =ₛ some τ → some (σ[x ↦ v]) =ₛ some (τ[x ↦ ↑v :: τ x]) := by
   intros _ y
   cases eq_or_ne x y
   · simp [‹x = y›]
   · simpa [‹x ≠ y›] using ‹σ=ₛτ› y
 
-lemma eq_states_INC {σ : LOOP.Store} {t : SCORE.State} {x : Ident} {v : ℕ} : some ([x ↦ v] σ) =ₛ t → some ([x ↦ v + 1] σ) =ₛ SCORE.eval (SCORE.Com.INC x) t := by
+lemma eq_states_INC {σ : LOOP.Store} {t : SCORE.State} {x : Ident} {v : ℕ} : some (σ[x ↦ v]) =ₛ t → some (σ[x ↦ v + 1]) =ₛ SCORE.eval (SCORE.Com.INC x) t := by
   intro
   cases t
   case some τ _ =>
     rw [SCORE.eval]
-    simp only [←‹some ([x ↦ v] σ) =ₛ some τ› x]
+    simp only [←‹some (σ[x ↦ v]) =ₛ some τ› x]
     intro y
     cases eq_or_ne x y
     · simp [‹x = y›]
-    · simpa [‹x ≠ y›] using ‹some ([x ↦ v] σ) =ₛ some τ› y
+    · simpa [‹x ≠ y›] using ‹some (σ[x ↦ v]) =ₛ some τ› y
   case none =>
     contradiction
 
