MasterThesis/LOOP/Proofs/Language.lean
@@ -5,21 +5,21 @@ import MasterThesis.LOOP.Language
 open LOOP Store
 
 @[simp]
-lemma update_same {s : Store} {x y : Ident} {v : Nat} : x = y → (update x v s) y = v := by
+lemma update_same {σ : Store} {x y : Ident} {v : Nat} : x = y → (σ[x ↦ v]) y = v := by
   intros
   unfold update
   apply if_pos
   assumption
 
 @[simp]
-lemma update_other {s : Store} {x y : Ident} {v : Nat} : x ≠ y → (update x v s) y = (s y) := by
+lemma update_other {σ : Store} {x y : Ident} {v : Nat} : x ≠ y → (σ[x ↦ v]) y = (σ y) := by
   intros
   unfold update
   apply if_neg
   assumption
 
 @[simp]
-lemma update_no_update {s : Store} {x : Ident} : (update x (s x) s) = s := by
+lemma update_no_update {σ : Store} {x : Ident} : (σ[x ↦ (σ x)]) = σ := by
   funext y
   cases eq_or_ne x y with
   | inl /- x = y -/ => rw[update_same ‹x = y›, ‹x = y›]
