MasterThesis/SCORE/Interpreter.lean
@@ -12,15 +12,15 @@ mutual
     | some σ =>
       match P with
       | SKIP    => s
-      | CON x   => some ([x ↦ (0 :: (σ x))] σ)
+      | CON x   => some (σ [x ↦ (0 :: (σ x))])
       | NOC x   => match (σ x).head? with
-                   | some 0 => some ([x ↦ (σ x).tail] σ)
+                   | some 0 => some (σ [x ↦ (σ x).tail])
                    | _      => none
       | DEC x   => match (σ x).head? with
-                   | some v => some ([x ↦ ((v - 1) :: (σ x).tail)] σ)
+                   | some v => some (σ [x ↦ ((v - 1) :: (σ x).tail)])
                    | none   => none
       | INC x   => match (σ x).head? with
-                   | some v => some ([x ↦ ((v + 1) :: (σ x).tail)] σ)
+                   | some v => some (σ [x ↦ ((v + 1) :: (σ x).tail)])
                    | none   => none
       | SEQ P Q => (eval Q) (eval P s)
       | FOR x P => match (σ x).head? with
@@ -35,14 +35,14 @@ mutual
       match P with
       | SKIP    => s
       | CON x   => match (σ x).head? with
-                   | some 0 => some ([x ↦ (σ x).tail] σ)
+                   | some 0 => some (σ [x ↦ (σ x).tail])
                    | _   => none
-      | NOC x   => some ([x ↦ (0 :: (σ x))] σ)
+      | NOC x   => some (σ [x ↦ (0 :: (σ x))])
       | DEC x   => match (σ x).head? with
-                   | some v => some ([x ↦ ((v + 1) :: (σ x).tail)] σ)
+                   | some v => some (σ [x ↦ ((v + 1) :: (σ x).tail)])
                    | none   => none
       | INC x   => match (σ x).head? with
-                   | some v => some ([x ↦ ((v - 1) :: (σ x).tail)] σ)
+                   | some v => some (σ [x ↦ ((v - 1) :: (σ x).tail)])
                    | none   => none
       | SEQ P Q => (evalI Q) (evalI P s)
       | FOR x P => match (σ x).head? with
