MasterThesis/SCORE/Proofs/Language.lean
@@ -19,40 +19,40 @@ theorem inv_inv (P : Com) : (inv (inv P)) = P := by
 namespace Store
 
 @[simp]
-lemma update_same {σ : Store} {x y : Ident} {l : List Int} : x = y → (update x l σ) y = l := by
+lemma update_same {σ : Store} {x y : Ident} {l : List Int} : x = y → (σ[x ↦ l]) y = l := by
   intros; simp only [if_pos ‹x = y›, update]
 
 @[simp]
-lemma update_other {σ : Store} {x y : Ident} {l : List Int} : x ≠ y → (update x l σ) y = σ y := by
+lemma update_other {σ : Store} {x y : Ident} {l : List Int} : x ≠ y → (σ[x ↦ l]) y = σ y := by
   intros; simp only [if_neg ‹x ≠ y›, update]
 
 @[simp]
-lemma update_shrink {σ : Store} {x : Ident} {l₁ l₂ : List Int} : (update x l₂ (update x l₁ σ)) = update x l₂ σ := by
+lemma update_shrink {σ : Store} {x : Ident} {l₁ l₂ : List Int} : σ[x ↦ l₁][x ↦ l₂] = σ[x ↦ l₂] := by
   funext y
   cases eq_or_ne x y with
   | inl /- x = y -/ => simp only [update_same ‹x = y›]
   | inr /- x ≠ y -/ => simp only [update_other ‹x ≠ y›]
 
 @[simp]
-lemma update_unchanged {σ : Store} {x : Ident} : update x (σ x) σ = σ := by
+lemma update_unchanged {σ : Store} {x : Ident} : σ[x ↦ (σ x)] = σ := by
   funext y
   cases eq_or_ne x y with
   | inl /- x = y -/ => rewrite [‹x = y›]; simp only [update_same]
   | inr /- x ≠ y -/ => simp only [update_other ‹x ≠ y›]
 
-lemma update_unchanged_cons {σ : Store} {x : Ident} {v : Int} : (σ x).head? = some v → update x (v :: (σ x).tail) σ = σ := by
+lemma update_unchanged_cons {σ : Store} {x : Ident} {v : Int} : (σ x).head? = v → σ[x ↦ (v :: (σ x).tail)]= σ := by
   intro
   funext y
   cases eq_or_ne x y with
   | inl /- x = y-/ =>
     rw [← ‹x = y›]
-    have : ([x ↦ (v :: (σ x).tail)] σ) x = (v :: (σ x).tail) := by
+    have : (σ[x ↦ (v :: (σ x).tail)]) x = (v :: (σ x).tail) := by
       { simp [‹x = y›]}; rw [this]
     have : v ∈ (σ x).head? := by
       { rw [Option.mem_def]; assumption }
     exact List.cons_head?_tail ‹v ∈ (σ x).head?›
   | inr /- x ≠ y-/ =>
-    have : ([x ↦ (v :: (σ x).tail)] σ) y = σ y := by
+    have : (σ[x ↦ (v :: (σ x).tail)]) y = σ y := by
       { simp [‹x ≠ y›] }; rw [this]
 
 end Store
